src/VMPanic.v
@@ -1,10 +1,8 @@
-Require Addressing CallStack Common GPR Flags isa.CoreSet State Steps.
-Import Addressing CallStack Common GPR Flags isa.CoreSet State Steps.
+Require Common isa.CoreSet.
+Import Common isa.CoreSet.
 
 Section Panics.
-  (**
-
-# Panic
+  (** # Panic
 
 **Panic** refers to a situation of irrecoverable error.
 It can occur for one of the following reasons:
@@ -17,8 +15,12 @@ It can occur for one of the following reasons:
 - Attempt to execute an invalid instruction.
 -
 Providing an integer value (with the tag cleared) instead of a pointer value (with the tag set) to an instruction that expects a tagged fat pointer value, e.g. [%OpPtrAdd].
+
+## Complete list of panic reasons
+
+The type [%reason] describes all situations where EraVM panics.
    *)
-  Inductive reason:=
+  Inductive reason :=
   | NotEnoughErgs
   | NotInKernelMode
   | ForbiddenInStaticMode
@@ -29,97 +31,9 @@ Providing an integer value (with the tag cleared) instead of a pointer value (wi
   | TriggeredExplicitly
   .
 
-  (**
-EraVM handles the panic situation as follows:
-
-- return from the current function signaling an error;
-- execute exception handler;
-- burn all ergs in current frame;
-- set OF flag;
-- restore depot and event queues to the state before external call (see [%gs_revertable]).
-- when returning from a far call, return no data.
-
-## Case 1: `panic` from near call
-
-1. Perform a [%rollback].
-2. Drop current frame with its ergs.
-3. Set PC to the exception handler of a dropped frame.
-4. Clear flags, and set OF.
-   *)
-  Inductive step_panic (why:reason) : smallstep :=
-  | step_PanicLocal_nolabel:
-    forall flags pages cf caller_stack regs gs gs' __,
-      let handler := active_exception_handler (InternalCall cf caller_stack) in
-      rollback (cf_saved_checkpoint cf) gs gs' ->
-      step_panic why
-                 {|
-                   gs_transient:= {|
-                                   gs_flags        := flags;
-                                   gs_callstack    := InternalCall cf caller_stack;
-                                   gs_regs         := regs;
-                                   gs_context_u128 := __;
-
-
-                                   gs_pages        := pages;
-                                 |};
-
-                   gs_global       := gs;
-                 |}
-                 {|
-                   gs_transient:= {|
-                                   gs_flags        := set_overflow flags_clear;
-                                   gs_regs         := regs_state_zero;
-                                   gs_callstack    := pc_set cf.(cf_exception_handler_location) caller_stack;
-                                   gs_context_u128 := zero128;
-
-                                   gs_pages        := pages;
-                                 |};
-
-                   gs_global       := gs'
-                 |}
-  (**
-## Case 2: `panic` from external call
-
-1. Perform a [%rollback].
-2. Drop current frame and its ergs
-3. Clear flags and set OF.
-4. Clear context register.
-5. Set PC to the exception handler address of a dropped frame.
-6. All storages are reverted to the state prior to the current contract call.
-7. Put an encoded zero-pointer into `R1` and tag `R1` as a pointer.
-
-   All other registers are zeroed. Registers `R2`, `R3` and `R4` are reserved
-   and may gain a special meaning in newer versions of EraVM.
-   *)
-  | step_PanicExt:
-    forall flags pages cf caller_stack __ regs (arg:in_reg) gs gs',
-      let cs0 := ExternalCall cf (Some caller_stack) in
-      rollback (cf_saved_checkpoint cf) gs gs' ->
-      step_panic why
-                 {|
-                   gs_transient := {|
-                                    gs_flags        := flags;
-                                    gs_callstack    := cs0;
-                                    gs_regs         := regs;
-                                    gs_context_u128 := __;
-
-
-                                    gs_pages        := pages;
-                                  |};
-
-                   gs_global       := gs;
-                 |}
-                 {|
-                   gs_transient := {|
-                                    gs_flags        := set_overflow flags_clear;
-                                    gs_regs         := regs_state_zero;
-                                    gs_callstack    := pc_set (active_exception_handler cs0) caller_stack;
-                                    gs_context_u128 := zero128;
-
-                                    gs_pages        := pages;
-                                  |};
-
-                   gs_global       := gs'
-                 |}
+  Inductive status :=
+  | NoPanic
+  | Panic : reason -> status
   .
+
 End Panics.
