src/sem/StepPanic.v
@@ -1,0 +1,103 @@
+Require Addressing CallStack Common GPR Flags isa.CoreSet State Steps VMPanic.
+Import Addressing CallStack Common GPR Flags isa.CoreSet State Steps VMPanic.
+
+Section StepPanic.
+  (** # Handling panics
+
+EraVM handles the panic situation as follows:
+
+- return from the current function signaling an error;
+- execute exception handler;
+- burn all ergs in current frame;
+- set OF flag;
+- restore depot and event queues to the state before external call (see [%gs_revertable]).
+- when returning from a far call, return no data.
+
+## Case 1: `panic` from near call
+
+1. Perform a [%rollback].
+2. Drop current frame with its ergs.
+3. Set PC to the exception handler of a dropped frame.
+4. Clear flags, and set OF.
+   *)
+  Inductive step_panic reason: smallstep :=
+  | step_PanicLocal_nolabel:
+    forall flags pages cf caller_stack regs gs gs' __,
+      let handler := active_exception_handler (InternalCall cf caller_stack) in
+      rollback (cf_saved_checkpoint cf) gs gs' ->
+      step_panic reason
+                 {|
+                   gs_transient:= {|
+                                   gs_flags        := flags;
+                                   gs_callstack    := InternalCall cf caller_stack;
+                                   gs_regs         := regs;
+                                   gs_context_u128 := __;
+                                   gs_status       := Panic reason;
+
+
+                                   gs_pages        := pages;
+                                 |};
+
+                   gs_global       := gs;
+                 |}
+                 {|
+                   gs_transient:= {|
+                                   gs_flags        := set_overflow flags_clear;
+                                   gs_regs         := regs_state_zero;
+                                   gs_callstack    := pc_set cf.(cf_exception_handler_location) caller_stack;
+                                   gs_context_u128 := zero128;
+                                   gs_status       := NoPanic;
+
+                                   gs_pages        := pages;
+                                 |};
+
+                   gs_global       := gs'
+                 |}
+  (**
+## Case 2: `panic` from external call
+
+1. Perform a [%rollback].
+2. Drop current frame and its ergs
+3. Clear flags and set OF.
+4. Clear context register.
+5. Set PC to the exception handler address of a dropped frame.
+6. All storages are reverted to the state prior to the current contract call.
+7. Put an encoded zero-pointer into `R1` and tag `R1` as a pointer.
+
+   All other registers are zeroed. Registers `R2`, `R3` and `R4` are reserved
+   and may gain a special meaning in newer versions of EraVM.
+   *)
+  | step_PanicExt:
+    forall flags pages cf caller_stack __ regs gs gs',
+      let cs0 := ExternalCall cf (Some caller_stack) in
+      rollback (cf_saved_checkpoint cf) gs gs' ->
+      step_panic reason
+                 {|
+                   gs_transient := {|
+                                    gs_flags        := flags;
+                                    gs_callstack    := cs0;
+                                    gs_regs         := regs;
+                                    gs_context_u128 := __;
+                                    gs_status       := Panic reason;
+
+
+                                    gs_pages        := pages;
+                                  |};
+
+                   gs_global       := gs;
+                 |}
+                 {|
+                   gs_transient := {|
+                                    gs_flags        := set_overflow flags_clear;
+                                    gs_regs         := regs_state_zero;
+                                    gs_callstack    := pc_set (active_exception_handler cs0) caller_stack;
+                                    gs_context_u128 := zero128;
+                                    gs_status       := NoPanic;
+
+                                    gs_pages        := pages;
+                                  |};
+
+                   gs_global       := gs'
+                 |}
+  .
+End StepPanic.
